STLCv0 abandoned bind. TypeBind & TrmBind should be different

Lp2lc/Active/STLC/Def.lean
@@ -1,15 +1,37 @@
 import Mathlib.Tactic
 import «Lp2lc».Active.Shared
 
-namespace Lp2lc.Active.STLC
+namespace Lp2lc.Active
+
+namespace Exp
+
+inductive TypLike (X: Type) : Type
+| _unknown: X -> TypLike X
+| all : TypLike X -- all-inclusive base type
+| arrow : X -> X -> TypLike X
+deriving Repr
+
+end Exp
+---
+namespace STLC
+
+class Sys
 
 mutual
+-- System extension, induction rule always cast input into output in either the same system or the most specific system that defined the rule
+-- AKA, Typ and Trm are always closed under rules/composition/induction
+-- e.g. using STLC rule can cast STLC Typ into STLC Typ, or F Typ into F Typ
+-- but using F rule can only cast both STLC/F Typ into F Typ
+-- this goes both ways
+-- the problem is that theorems are defined for types (including wrapper), not rules
 -- Basic (pre)types --
 inductive TypLike {X: Type} : Type
 | _unknown: X -> TypLike
 | all : TypLike -- all-inclusive base type
 | arrow : TypLike -> TypLike -> TypLike
 deriving Repr
+
+
 
 -- Defining (pre)terms by recursion --
 inductive TrmLike {X: Type} : Type
@@ -21,7 +43,15 @@ inductive TrmLike {X: Type} : Type
 deriving Repr
 end
 
-abbrev Typ {X: Type} : Type := { T : TypLike (X := X) // ∀ x : X, T ≠ TypLike._unknown x }
-abbrev Trm {X: Type} : Type := { T : TrmLike (X := X) // ∀ x : X, T ≠ TrmLike._unknown x }
+abbrev Typ {X: Type} := { T : TypLike (X := X) // ∀ x : X, T ≠ TypLike._unknown x }
+abbrev Trm {X: Type} := { T : TrmLike (X := X) // ∀ x : X, T ≠ TrmLike._unknown x }
 
-end Lp2lc.Active.STLC
+end STLC
+
+namespace F
+
+class Sys extends STLC.Sys
+
+end F
+
+end Lp2lc.Active
